[kernel-f11n] Fix statement typing and complete proof of statement typing consistency.
Previously, we inferred the return type of statements in a way that made it
impossible to prove the statement typing consistency. Now, we use just the
stated return type for checking statements.

The proofs of statement typing are complete, except for one result generalizing
the expression typing consistency result to multiple variables changing; this
result is obvious to see directly from the provided lemmas but very tedious to
prove in Coq.

Bug:
Change-Id: I0bbcfb613df7510015f278fa85021ba0b3e57503
Reviewed-on: https://dart-review.googlesource.com/9020
Reviewed-by: Dmitry Stefantsov <dmitryas@google.com>

pkg/kernel/coq/Common.v
@@ -125,6 +125,19 @@ Module ListExtensions.
     induction l; crush.
   Qed.
 
+  Fixpoint list_all {A} (f : A -> Prop) (l : list A) :=
+    match l with
+    | nil => True
+    | (x::xs) => f x /\ list_all f xs
+    end.
+
+  Lemma forall_list_all : forall A P (l : list A), Forall P l <-> list_all P l.
+    intros.
+    apply conj.
+    intro f.
+    induction f; crush.
+    induction l; crush.
+  Qed.
 End ListExtensions.
 
 (* These could be generalized and factored into a functor, like FMapFacts, but
@@ -132,6 +145,7 @@ End ListExtensions.
 Module MoreNatMapFacts.
 
 Module N := Coq.Arith.PeanoNat.Nat.
+
 Lemma add_3 {A} : forall m x (y y' : A), NatMap.MapsTo x y m /\ NatMap.MapsTo x y' m -> y = y'.
   intuition.
   set (Fx := NatMap.find x m).
@@ -139,6 +153,22 @@ Lemma add_3 {A} : forall m x (y y' : A), NatMap.MapsTo x y m /\ NatMap.MapsTo x 
   pose proof (NatMap.find_1 H0).
   pose proof (NatMap.find_1 H1).
   crush.
+Qed.
+
+Lemma maps_in_mapsto :
+  forall A (m : NatMap.t A) key,
+  NatMap.In key m ->
+  exists el, NatMap.MapsTo key el m.
+Proof.
+  intros.
+  pose proof (NatMapFacts.find_mapsto_iff m key).
+  pose proof (NatMapFacts.in_find_iff m key).
+    unfold iff in H1. destruct H1 as [H1a H1b].
+  pose proof (H1a H).
+  destruct (NatMap.find key m) eqn:?.
+    exists a. pose proof (H0 a). unfold iff in H2. destruct H2 as [H2a H2b].
+      apply H2b. congruence.
+    contradiction.
 Qed.
 
 End MoreNatMapFacts.
