pkg/kernel/coq/CommonTactics.v
@@ -41,9 +41,22 @@ Ltac extract_head_2 term H varid eqid :=
 Ltac extract_head_1 term H varid := let eqid := fresh varid "Eq" in extract_head_2 term H varid eqid.
 Ltac extract_head_0 term H := let varid := fresh H in extract_head_1 term H varid.
 
+Ltac extract_head_goal_2 term varid eqid :=
+  match goal with
+  | [ |- context[term ?X] ] => extract_head_goal_2 (term X) varid eqid
+  | [ |- context[term] ] => remember term as varid eqn:eqid
+  end.
+
+Ltac extract_head_goal_1 term varid := let eqid := fresh varid "Eq" in extract_head_goal_2 term varid eqid.
+Ltac extract_head_goal_0 term := let varid := fresh "G" in extract_head_goal_1 term varid.
+
 Tactic Notation "extract_head" constr(term) "in" constr(H) := extract_head_0 term H.
 Tactic Notation "extract_head" constr(term) "in" constr(H) "as" ident(name) := extract_head_1 term H name.
 Tactic Notation "extract_head" constr(term) "in" constr(H) "as" ident(name) "," ident(name2) := extract_head_2 term H name name2.
+
+Tactic Notation "extract_head" constr(term) := extract_head_goal_0 term.
+Tactic Notation "extract_head" constr(term) "as" ident(name) := extract_head_goal_1 term name.
+Tactic Notation "extract_head" constr(term) "as" ident(name) "," ident(name2) := extract_head_goal_2 term name name2.
 
 Ltac continue_with H :=
   match type of H with
